Propagate changes to types of arrays and records.

rocq-osiris/theories/program_logic/rules/array_rules.v
@@ -7,7 +7,7 @@ From osiris.logic Require Import list_z big_opLZ.
 
 (** This file defines array resource predicates and [imp] rules for array expressions. *)
 
-Definition array : Type := syntax.block.
+Definition array : Type := syntax.array.
 
 Section array_resources.
 
@@ -139,48 +139,14 @@ Section array_reasoning.
   (** General [as_array] rule.  Given that the postcondition of [m] implies
       [isBlockLocs a ls] for some [a] and [ls], the [load_block] step is
       discharged automatically and [Φ ls] is delivered. *)
-  Lemma imp_as_array {ζ} {Φ : list loc → iProp Σ} (Φ1 : array → iProp Σ) (m : microvx) :
-    imp m @ E <|Ψ|> ⟨⟨ ζ ⟩⟩ {{ Φ1 }} -∗
-    (∀ (a : array), Φ1 a -∗ ∃ ls, ▷ isBlockLocs a ls ∗ Φ ls) -∗
+  Lemma imp_as_array {ζ} {Φ : array → iProp Σ} (m : microvx) :
+    imp m @ E <|Ψ|> ⟨⟨ ζ ⟩⟩ {{ Φ }} -∗
     imp as_array m @ E <|Ψ|> ⟨⟨ ζ ⟩⟩ {{ Φ }}.
-  Proof.
-    iIntros "Hm H".
-    iApply (imp_bind with "Hm").
-    iIntros (a) "HΦ1".
-    iDestruct ("H" with "HΦ1") as "(%ls & #Harr & HΦ)".
-    iApply (imp_bind with "[Harr]").
-    { iApply (imp_load_block_ghost with "Harr"). }
-    iIntros ([? ?]) "->".
-    iApply (imp_ret with "HΦ"). encode.
-  Qed.
-
-  (** [as_array] rule for a pre-existing array.  Use when [isBlockLocs a ls] is
-      already in context and [m] reduces to the array address [a]. *)
-  Lemma imp_as_array_isBlockLocs {ζ} {Φ : list loc → iProp Σ} (a : syntax.block) ls (m : microvx) :
-    ▷ isBlockLocs a ls -∗
-    imp m @ E <|Ψ|> ⟨⟨ ζ ⟩⟩ {{ λ a', ⌜a' = a⌝ }} -∗
-    Φ ls -∗
-    imp as_array m @ E <|Ψ|> ⟨⟨ ζ ⟩⟩ {{ Φ }}.
-  Proof.
-    iIntros "#Harr Hm HΦ".
-    iApply (imp_as_array (λ a', ⌜a' = a⌝)%I with "Hm").
-    iIntros (a') "->".
-    iExists ls. iFrame "#∗".
-  Qed.
-
-  (** [as_array] rule for a freshly allocated array.  Use when [m] allocates
-      an array, producing [ownArray a ls xs]; the full ownership is preserved
-      in the postcondition together with any additional frame [R a xs]. *)
-  Lemma imp_as_array_ownArray `{Encode A} {ζ}
-      {R : array → list A → iProp Σ} (m : microvx) :
-    imp m @ E <|Ψ|> ⟨⟨ ζ ⟩⟩ {{ λ a, ∃ (xs : list A), a ↦∗ xs ∗ R a xs }} -∗
-    imp as_array m @ E <|Ψ|> ⟨⟨ ζ ⟩⟩ {{ λ ls, ∃ a xs, a ↦∗ xs ∗ R a xs }}.
   Proof.
     iIntros "Hm".
-    iApply (imp_as_array (λ a, ∃ xs, a ↦∗ xs ∗ R a xs)%I with "Hm").
-    iIntros (a) "(%xs & Hown & $)".
-    iPoseProof (ownArray_isBlockLocs with "Hown") as "(%ls & #Ha & %hlen)".
-    iFrame "Hown". iExists ls. iFrame "#".
+    iApply (imp_bind with "Hm").
+    iIntros (a) "HΦ".
+    iApply (imp_ret with "HΦ"). encode.
   Qed.
 
   Lemma imp_EArrayLit `{Encode A} {ζ} (Φs : list (A → iProp Σ)) es :
@@ -227,15 +193,16 @@ Section array_reasoning.
   Qed.
 
   Lemma imp_EArrayLength' {ζ} (ls : list loc) e :
-    imp eval η e @ E <|Ψ|> ⟨⟨ ζ ⟩⟩ {{ λ (a : syntax.block), isBlockLocs a ls }} -∗
+    imp eval η e @ E <|Ψ|> ⟨⟨ ζ ⟩⟩ {{ λ (a : array), isBlockLocs a ls }} -∗
     imp eval η (EArrayLength e) @ E <|Ψ|> ⟨⟨ ζ ⟩⟩ {{ λ n, ⌜n = length ls⌝ }}.
   Proof.
     iIntros "He". simpl_eval.
     iApply (imp_bind with "[He] [-]").
-    - set_postcondition (λ ls', ⌜ls'=ls⌝)%I.
-      iApply (imp_as_array with "He").
-      iIntros (a) "#Harr". by iFrame "#".
-    - iIntros (ls') "->". iApply imp_ret; first encode. auto.
+    { iApply (imp_as_array with "He"). }
+    iIntros (a) "#HBlock".
+    iApply imp_bind.
+    { iApply (imp_load_block_ghost with "HBlock"). }
+    iIntros ((t & ls')) "->". iApply imp_ret; first encode. auto.
   Qed.
 
   Lemma imp_EArrayLength `{Encode A} {ζ} dq (xs : list A) e :
@@ -244,11 +211,14 @@ Section array_reasoning.
   Proof.
     iIntros "He". simpl_eval.
     iApply (imp_bind with "[He] [-]").
-    - set_postcondition (λ ls, ⌜length ls = length xs⌝)%I.
-      iApply (imp_as_array with "He").
-      iIntros (a) "Hown".
-      iPoseProof (ownArray_isBlockLocs with "Hown") as "(% & $ & $)".
-    - iIntros (ls) "<-". iApply imp_ret; first encode. auto.
+    { iApply (imp_as_array with "He"). }
+    iIntros (a) "Hslice".
+    iPoseProof (ownArray_isBlockLocs with "Hslice") as "(%ls & #Hblock & %Hbounds)".
+    iApply imp_bind.
+    { iApply (imp_load_block_ghost with "Hblock"). }
+    iIntros ((t & ls')) "->".
+    iApply imp_ret; first encode.
+    auto.
   Qed.
 
   Lemma imp_EArrayMake `{Encode A} {ζ} {e1 e2} (n : Z) (Φ : A → iProp Σ) :
@@ -320,7 +290,7 @@ Section array_reasoning.
       revert Hlen. length. lia.
   Qed.
 
-  Lemma slice_insert_acc `{Encode A, Inhabited A} (i j : Z) (a : syntax.block) (xs : list A) (ls : list loc) :
+  Lemma slice_insert_acc `{Encode A, Inhabited A} (i j : Z) (a : array) (xs : list A) (ls : list loc) :
     j ≤ i < j + length xs →
     a ↦∗[j] xs -∗
     isBlockLocs a ls -∗
@@ -338,7 +308,7 @@ Section array_reasoning.
     iFrame "∗#%".
   Qed.
 
-  Lemma slice_lookup_acc `{Encode A, Inhabited A} (i j : Z) (a : syntax.block) dq (xs : list A) (ls : list loc) :
+  Lemma slice_lookup_acc `{Encode A, Inhabited A} (i j : Z) (a : array) dq (xs : list A) (ls : list loc) :
     j ≤ i < j + length xs →
     a ↦∗[j]{dq} xs -∗
     isBlockLocs a ls -∗
@@ -355,7 +325,7 @@ Section array_reasoning.
     iFrame "∗#%".
   Qed.
 
-  Lemma imp_EArrayGet2 `{Encode A, Inhabited A} {Φ : A → iProp Σ} {ζ} (Φ2 : Z → iProp Σ) e1 e2 (a : syntax.block) ls :
+  Lemma imp_EArrayGet2 `{Encode A, Inhabited A} {Φ : A → iProp Σ} {ζ} (Φ2 : Z → iProp Σ) e1 e2 (a : array) ls :
     ▷ isBlockLocs a ls -∗
     imp eval η e1 @ E <|Ψ|> ⟨⟨ ζ ⟩⟩ {{ λ a', ⌜a'=a⌝ }} -∗
     imp eval η e2 @ E <|Ψ|> ⟨⟨ ζ ⟩⟩ {{ Φ2 }} -∗
@@ -367,7 +337,7 @@ Section array_reasoning.
   Proof.
     iIntros "#Ha He1 He2 P". simpl_eval.
     iApply (imp_bind_par with "[He1] [He2]").
-    - iApply (imp_as_array_isBlockLocs a ls (Φ := λ ls', ⌜ls' = ls⌝%I) with "Ha He1"). auto.
+    - iApply (imp_as_array with "He1").
     - iApply (imp_as_int with "He2").
     - iIntros (? i) "-> HΦ2".
       iDestruct ("P" with "HΦ2") as
@@ -378,6 +348,8 @@ Section array_reasoning.
       iPoseProof (isBlockLocs_length with "Ha") as "%Hlenls".
 
       simpl.
+      iApply imp_bind. iApply (imp_load_block_ghost with "Ha").
+      iIntros ((t & ls')) "-> /=".
       rewrite signed_repr; last representable.
       rewrite list_lookup_lookup_total_valid; last lia.
       (* Subgoal: [load (a !!! i)] *)
@@ -389,7 +361,7 @@ Section array_reasoning.
       iApply ("Hslice" with "Hl").
   Qed.
 
-  Lemma imp_EArrayGet' `{Encode A, Inhabited A} {ζ} (a : syntax.block) (i j : Z) dq (xs : list A) e1 e2 :
+  Lemma imp_EArrayGet' `{Encode A, Inhabited A} {ζ} (a : array) (i j : Z) dq (xs : list A) e1 e2 :
     ⌜j ≤ i < j + length xs⌝ -∗
     ▷ a ↦∗[j]{dq} xs -∗
     imp eval η e1 @ E <|Ψ|> ⟨⟨ ζ ⟩⟩ {{ λ a', ⌜a' = a⌝ }} -∗
@@ -427,11 +399,11 @@ Section array_reasoning.
   Qed.
 
   Lemma imp_EArraySet2 `{Encode A, Inhabited A} {Φ : unit → iProp Σ} {ζ}
-    (Φ3 : A → iProp Σ) (Φ1 : array → list loc → iProp Σ) (Φ2 : Z → iProp Σ) e1 e2 e3 :
-    imp eval η e1 @ E <|Ψ|> ⟨⟨ ζ ⟩⟩ {{ λ (a : array), ∃ ls, ▷ isBlockLocs a ls ∗ Φ1 a ls }} -∗
+    (Φ3 : A → iProp Σ) (Φ1 : array → iProp Σ) (Φ2 : Z → iProp Σ) e1 e2 e3 :
+    imp eval η e1 @ E <|Ψ|> ⟨⟨ ζ ⟩⟩ {{ Φ1 }} -∗
     imp eval η e2 @ E <|Ψ|> ⟨⟨ ζ ⟩⟩ {{ Φ2 }} -∗
     imp eval η e3 @ E <|Ψ|> ⟨⟨ ζ ⟩⟩ {{ Φ3  }} -∗
-    (∀ a ls i y, Φ1 a ls -∗ Φ2 i -∗ Φ3 y -∗
+    (∀ a i y, Φ1 a -∗ Φ2 i -∗ Φ3 y -∗
                  ∃ j xs,
                    ▷ (⌜j ≤ i < j + length xs⌝ ∗ a ↦∗[j] xs) ∗
                    ▷ (a ↦∗[j] (<[i - j := y]> xs) -∗ Φ ())) -∗
@@ -439,33 +411,28 @@ Section array_reasoning.
   Proof.
     iIntros "He1 He2 He3 P". simpl_eval.
     iApply (imp_bind_par (A2:=(Z * A)) with "[He1] [He2 He3]").
-    { set_postcondition (λ ls, ∃ a, ▷ isBlockLocs a ls ∗ Φ1 a ls)%I.
-      iApply (imp_as_array with "He1").
-      iIntros (l) "(% & #$ & $)". }
+    { iApply (imp_as_array with "He1"). }
     { iApply (imp_par with "[He2] He3").
       iApply (imp_as_int with "He2"). }
-    iIntros (ls (i & y)) "(%a & #Ha & HΦ1) (HΦ2 & HΦ3)".
-    iDestruct ("P" with "HΦ1 HΦ2 HΦ3")
-      as "(%j & %xs & >(%Hle & Hslice) & HΦ)".
+    iIntros (a (i & y)) "HΦ1 (HΦ2 & HΦ3)".
+    iDestruct ("P" with "HΦ1 HΦ2 HΦ3") as
+        "(%j & %xs & Hslice & HΦ)". iNext.
+    iDestruct "Hslice" as "(%Hbound & Hslice)".
+    iPoseProof (isSlice_isBlockLocs with "Hslice") as "(%ls & #Hblock & %Hbounds)".
+    iPoseProof (isBlockLocs_length with "Hblock") as "%Hlen'".
 
-    iDestruct "Hslice" as "(% & #Ha' & %Hlen & Hslice)".
-    iNext.
-    iPoseProof (isBlockLocs_valid with "Ha Ha'") as "->".
-    iPoseProof (isBlockLocs_length with "Ha") as "%Hlen'".
-
-    simpl.
+    iApply imp_bind. { iApply (imp_load_block_ghost with "Hblock"). }
+    iIntros ((t & ls')) "-> /=".
     rewrite signed_repr; last representable.
     rewrite list_lookup_lookup_total_valid; last lia.
     (* Subogal: [store (a !!! i) #y] *)
-    iPoseProof (big_sepLZ2_insert_seg_acc i with "Hslice")
-      as "(Hl & Hslice)"; try lia.
+    iPoseProof (slice_insert_acc i with "Hslice Hblock") as "(Hl & Hslice)".
+    lia.
 
     iApply (imp_store' with "Hl").
     iIntros "!> Hl".
-    iApply "HΦ". iFrame "Ha'". length. iFrame "%".
-    iSpecialize ("Hslice" with "Hl").
-    update.
-    iApply "Hslice".
+    iApply "HΦ".
+    iApply ("Hslice" with "Hl").
   Qed.
 
   Lemma imp_EArraySet' `{Encode A, Inhabited A} {ζ}
@@ -480,15 +447,11 @@ Section array_reasoning.
   Proof.
     iIntros (Hbound) "Hslice He1 He2 He3".
     iDestruct "Hslice" as "(%ls & #Harr & >%Hlenls & slice)".
-    iApply (imp_EArraySet2 with "[He1] He2 He3").
-    { set_postcondition (λ a', ∃ ls', _ ∗ ⌜a' = a⌝ ∗ ⌜ls' = ls⌝)%I.
-      iApply (imp_wand with "He1").
-      iIntros (?) "->". iFrame "Harr". auto. }
-    iIntros (??? y) "(-> & ->) -> HΦ".
+    iApply (imp_EArraySet2 with "He1 He2 He3").
+    iIntros (???) "-> -> HΦ".
     iExists j, xs. iSplitL "slice".
     - iFrame. iFrame "%#".
-    - iIntros "!> $".
-      iFrame.
+    - iIntros "!> $". iFrame.
   Qed.
 
   Lemma imp_EArraySet `{Encode A, Inhabited A} {ζ}
